theories/simulations/ctxrefine/BehFacts.v
@@ -1,0 +1,44 @@
+From CRIS.common Require Import Common ConcRA.
+From CRIS.modules Require Import Mod LMod.
+From CRIS.simulations.gsim Require Import GSimAdequacy.
+From CRIS.simulations.lsim Require Import LSimAdequacy.
+From CRIS.simulations.msim Require Import MSimCommon ISimFacts ISimAdequacy.
+From CRIS.simulations.ctxrefine Require Import CtxRefine.
+
+Section MOD_BEHAVIOR.
+
+  Context `{!crisG Γ Σ α β τ _S _I}.
+
+  Lemma Beh_intro
+    M t r
+    (WF : Mod.wf M)
+    (BEH : Beh.of_itree (LMod.compile (Mod.to_lmod M r) tt↑) t)
+    : Own r ∗ winv (∅,∅) ⊢ Beh M t.
+  Proof.
+    eapply entails_pointwise. intros rt Vrt Hrt.
+    eapply Own_general_completeness. rewrite Beh_unseal.
+    intros rt' Vrt' LE.
+    assert (REFL : ISim.ISim.t closed M M emp IstEq).
+    { eapply ISim_refl; et. }
+    eapply (ISim_adequacy _ _ rt' r) in REFL; et.
+    2:{
+      iIntros "H". iModIntro.
+      iPoseProof (Own_extends with "H") as "H"; et.
+      iDestruct (Hrt with "H") as "[$ $]".
+    }
+    eapply (lsim_adequacy _ _ (tt↑)) in REFL.
+    eapply gsim_adequacy with (x0 := t) in REFL; et.
+  Qed.
+
+  Lemma Beh_elim
+    M t r
+    (BEH : Own r ⊢ Beh M t)
+    : forall r', ✓ r' -> r ≼ r' -> Beh.of_itree (LMod.compile (Mod.to_lmod M r) tt↑) t.
+  Proof.
+    intros r' Vr' LE.
+    assert (Vr : ✓ r) by (eapply cmra_valid_included; et).
+    eapply Own_general_soundness in BEH; et.
+    rewrite Beh_unseal in BEH. eapply BEH; et.
+  Qed.
+
+End MOD_BEHAVIOR.
